More locally nameless stuff

Chapter4.v
@@ -18,8 +18,10 @@ Require Import Coq.ZArith.ZArith_dec.
 Require Import Coq.Classes.EquivDec.
 Require Import Omega.
 
+Require Import WrengrUtil.Relations.Core.
 Require Import WrengrUtil.CoqExtras.ListSet.
 Require Import LNVar.
+Require Import LNVarMap.
 
 (* For [le_dec] and [lt_dec] *)
 Require Import Chapter1.
@@ -134,6 +136,7 @@ Inductive reduce_fb_db : db_exp -> db_exp -> Prop :=
         , reduce_fb_db e3 e3'
         -> reduce_fb_db (DBIf e1 e2 e3) (DBIf e1 e2 e3')
     .
+(* TODO: do we want to add hints about using these as intro rules? *)
 
 End STLC_with_De_Bruijn_Indices.
 
@@ -223,11 +226,14 @@ Fixpoint FV (e:exp) : set Var :=
 
 End STLC_with_Locally_Nameless.
 
+Notation "x \freshin e" := (x \notin (FV e))
+    (at level 68, no associativity) :listset_scope.
+
 
 (* ~~~~~~~~~~~~~~~~~~~~~~~~~~~~~~~~~~~~~~~~~~~~~~~~~~~~~~~~~~ *)
 Section Dynamic_Semantics_via_an_Interpreter.
 
-(** Substitution for local/bound-vars. Replace [BVar j] by [e] in [f]. *)
+(** Substitution for local/bound-vars. Replace [BVar j] by [e] in [f]. The [∆∆e·f] specialization is called ``opening'' (or [openTerm] in the theorems); and the [∆x·f] specialization is called ``variable opening'' (or [openVar] in the theorems). *)
 Fixpoint bsubst (j:nat) (e:exp) (f:exp) : exp :=
     match f with
     | Const c      => Const c
@@ -239,8 +245,14 @@ Fixpoint bsubst (j:nat) (e:exp) (f:exp) : exp :=
     | AppE e1 e2   => AppE (bsubst j e e1) (bsubst j e e2)
     end.
 (* Notation was ("{_\<rightarrow>_}_" [54,54,54]53) in Isabelle/HOL *)
+(* HACK: we use double braces instead of single braces to avoid conflict with the notation for, e.g., sumbool. *)
 Notation "{{ j ~> e }} f" := (bsubst j e f)
-    (at level 0, i at level 99, right associativity) :exp_scope.
+    (at level 0, j at level 99, right associativity) :exp_scope.
+(* Caveat: wide unicode characters like [·] can be especially problematic to display in the terminal... *)
+Notation "∆∆ e · f"     := (bsubst 0 e f)
+    (at level 67, right associativity) :exp_scope.
+Notation "∆ x · f"      := (bsubst 0 (FVar x) f)
+    (at level 67, right associativity) :exp_scope.
 
 
 (** Substitution for names/free-vars. Replace [FVar x] by [e] in [f]. *)
@@ -255,7 +267,8 @@ Fixpoint subst (x:Var) (e:exp) (f:exp) : exp :=
     | AppE e1 e2   => AppE (subst x e e1) (subst x e e2)
     end.
 (* Notation was ("[_\<mapsto>_] _" [72,72,72]71) in Isabelle/HOL *)
-Notation "[ x ~> e ] f" := (subst x e f)
+(* HACK: we use double brackets instead of single braces to avoid conflict with the notation for, e.g., lists. *)
+Notation "[[ x ~> e ]] f" := (subst x e f)
     (at level 0, x at level 99, right associativity) :exp_scope.
 
 
@@ -289,50 +302,29 @@ Proof.
 Qed.
 
 
-Definition VarMap A := list (Var * A).
-Definition env  := VarMap exp.
+Definition env := VarMap Var exp.
+Implicit Type ρ : env.
 
 
 (* TODO: notation "[_] _" [72,72]71 *)
-Fixpoint msubst (rho : env) (e : exp) : exp :=
-    match rho with
-    | nil         => e
-    | (x,v)::rho' => msubst rho' (subst x v e)
+Fixpoint msubst (ρ : env) (e : exp) : exp :=
+    match ρ with
+    | nil       => e
+    | (x,v)::ρ' => msubst ρ' (subst x v e)
     end.
 
 
-Definition VarMap_dom : forall {A}, VarMap A -> set Var :=
-    fun A =>
-        list_rect (fun _ => set Var)
-            \{}
-            (fun ab _ r => fst ab \a r).
-
-Definition env_dom := VarMap_dom exp.
-
-
-(* TODO: just return a list? use a notation instead in order to abstract over [eq_A_dec]? *)
-Definition assoc_dom
-    {A} (eq_A_dec : forall x y:A, {x = y} + {x <> y})
-    {B}
-    (xs : list (A*B))
-    : set A :=
-        list_to_set A eq_A_dec
-            (list_rect (fun _ => set A)
-                nil
-                (fun ab _ r => fst ab :: r)
-                xs).
-
-
+(* Caveat: displaying unicode characters like [ρ] might be a problem depending on your terminal... *)
 Lemma msubst_id :
-    forall rho e,
-    (forall x, x \notin (env_dom rho \n FV e)) ->
-    msubst rho e = e.
+    forall ρ e,
+    (forall x, x \notin (assoc_dom ρ \n FV e)) ->
+    msubst ρ e = e.
 Proof.
-  intro rho; induction rho; simpl; intros e H.
+  intro ρ; induction ρ; simpl; intros e H.
     reflexivity.
     
     destruct a; simpl in *.
-    rewrite IHrho.
+    rewrite IHρ.
       apply subst_id.
       intro; apply (H v).
       solve [auto with listset].
@@ -473,168 +465,269 @@ Proof.
       apply IHm'; auto.
 Qed.
 
-  
+End Dynamic_Semantics_via_an_Interpreter.
+
+(* HACK: have to repeat notations once we close the section *)
+Notation "{{ j ~> e }} f" := (bsubst j e f)
+    (at level 0, j at level 99, right associativity) :exp_scope.
+Notation "∆∆ e · f"     := (bsubst 0 e f)
+    (at level 67, right associativity) :exp_scope.
+Notation "∆ x · f"      := (bsubst 0 (FVar x) f)
+    (at level 67, right associativity) :exp_scope.
+Notation "[[ x ~> e ]] f" := (subst x e f)
+    (at level 0, x at level 99, right associativity) :exp_scope.
+
+
+(* ~~~~~~~~~~~~~~~~~~~~~~~~~~~~~~~~~~~~~~~~~~~~~~~~~~~~~~~~~~ *)
+Section Reduction_Semantics.
+Open Scope exp_scope. (* need to reopen since the old section was closed *)
+
+(** Abstract [FVar x] as [BVar i] in [e]. The inverse of [bsubst],
+    as it were. For a conventional named lambda, you can use [Lam(∇x·e)]. *)
+Fixpoint close (j:nat) (x:Var) (e:exp) : exp :=
+    match e with
+    | Const c      => Const c
+    | Prim p e'    => Prim p (close j x e')
+    | IfE e1 e2 e3 => IfE (close j x e1) (close j x e2) (close j x e3)
+    | FVar y       => if equiv_dec x y then BVar j else FVar y
+    | BVar k       => BVar k
+    | LambdaE e'   => LambdaE (close (S j) x e')
+    | AppE e1 e2   => AppE (close j x e1) (close j x e2)
+    end.
+(* Notation was ("{_\<leftarrow>_}_" [54,54,54] 53) in Isabelle/HOL *)
+Notation "{{ j <~ x }} e" := (close j x e)
+    (at level 0, j at level 99, right associativity) :exp_scope.
+Notation "∇ x · e"      := (close 0 x e)
+    (at level 67, right associativity) :exp_scope.
+
+
+(* Notation was (infix "\<longmapsto>fb" 70) in Isabelle/HOL *)
+Inductive reduce_fb : exp -> exp -> Prop :=
+    | full_beta
+        : forall e e'
+        , reduce_fb (AppE (LambdaE e) e') (∆∆e'·e)
+    | c_lambda
+        (* N.B., for soundness sake, beware how [x] is quantified! *)
+        : forall x e e'
+        ,  x \freshin e
+        -> reduce_fb (∆x·e)  e'
+        -> reduce_fb (LambdaE e) (LambdaE (∇x·e'))
+    | c_app1_fb
+        : forall e1 e1' e2
+        ,  reduce_fb e1 e1'
+        -> reduce_fb (AppE e1 e2) (AppE e1' e2)
+    | c_app2_fb
+        : forall e1 e2 e2'
+        ,  reduce_fb e2 e2'
+        -> reduce_fb (AppE e1 e2) (AppE e1 e2')
+    | r_prim_fb
+        : forall p c c'
+        ,  eval_prim p c = Result c'
+        -> reduce_fb (Prim p (Const c)) (Const c')
+    | c_prim_fb
+        : forall p e e'
+        ,  reduce_fb e e'
+        -> reduce_fb (Prim p e) (Prim p e')
+    | r_if_true_fb
+        : forall e2 e3
+        , reduce_fb (IfE (Const (BoolC true)) e2 e3) e2
+    | r_if_false_fb
+        : forall e2 e3
+        , reduce_fb (IfE (Const (BoolC false)) e2 e3) e3
+    | c_if1_fb
+        : forall e1 e1' e2 e3
+        ,  reduce_fb e1 e1'
+        -> reduce_fb (IfE e1 e2 e3) (IfE e1' e2 e3)
+    | c_if2_fb
+        : forall e1 e2 e2' e3
+        ,  reduce_fb e2 e2'
+        -> reduce_fb (IfE e1 e2 e3) (IfE e1 e2' e3)
+    | c_if3_fb
+        : forall e1 e2 e3 e3'
+        ,  reduce_fb e3 e3'
+        -> reduce_fb (IfE e1 e2 e3) (IfE e1 e2 e3')
+    .
+(* TODO: do we want to add hints about using these as intro rules? *)
+
+Fixpoint val (e:exp) : Prop :=
+    match e with
+    | Const _   => True
+    | LambdaE _ => True
+    | _         => False
+    end.
+
+
+(* notation was (infix "\<longmapsto>" 70) in Isabelle/HOL *)
+Inductive reduce_bv : exp -> exp -> Prop :=
+    | beta_bv
+        : forall v e
+        ,  val v
+        -> reduce_bv (AppE (LambdaE e) v) (∆∆v·e)
+    | c_app1_bv
+        : forall e1 e1' e2
+        ,  reduce_bv e1 e1'
+        -> reduce_bv (AppE e1 e2) (AppE e1' e2)
+    | c_app2_bv
+        : forall v e2 e2'
+        ,  val v
+        -> reduce_bv e2 e2'
+        -> reduce_bv (AppE v e2) (AppE v e2')
+    | r_prim_bv
+        : forall p c c'
+        ,  eval_prim p c = Result c'
+        -> reduce_bv (Prim p (Const c)) (Const c')
+    | c_prim_bv
+        : forall p e e'
+        ,  reduce_bv e e'
+        -> reduce_bv (Prim p e) (Prim p e')
+    | r_if_true_bv
+        : forall e2 e3
+        , reduce_bv (IfE (Const (BoolC true)) e2 e3) e2
+    | r_if_false_bv
+        : forall e2 e3
+        , reduce_bv (IfE (Const (BoolC false)) e2 e3) e3
+    | c_if_bv
+        : forall e1 e1' e2 e3
+        ,  reduce_bv e1 e1'
+        -> reduce_bv (IfE e1 e2 e3) (IfE e1' e2 e3)
+    .
+(* TODO: do we want to add hints about using these as intro rules? *)
+
+(* notation was (infix "\<longmapsto>*" 70) *)
+Definition reduces_bv := RTC_opt reduce_bv.
+
+
+(* notation was (infix "\<longmapsto>bn" 70) *)
+Inductive reduce_bn : exp -> exp -> Prop :=
+    | beta_bn
+        : forall e e'
+        , reduce_bn (AppE (LambdaE e) e') (∆∆e'·e)
+    | c_app_bn
+        : forall e1 e1' e2
+        ,  reduce_bn e1 e1'
+        -> reduce_bn (AppE e1 e2) (AppE e1' e2)
+    | r_prim_bn
+        : forall p c c'
+        ,  eval_prim p c = Result c'
+        -> reduce_bn (Prim p (Const c)) (Const c')
+    | c_prim_bn
+        : forall p e e'
+        ,  reduce_bn e e'
+        -> reduce_bn (Prim p e) (Prim p e')
+    | r_if_true_bn
+        : forall e2 e3
+        , reduce_bn (IfE (Const (BoolC true)) e2 e3) e2
+    | r_if_false_bn
+        : forall e2 e3
+        , reduce_bn (IfE (Const (BoolC false)) e2 e3) e3
+    | c_if_bn
+        : forall e1 e1' e2 e3
+        ,  reduce_bn e1 e1'
+        -> reduce_bn (IfE e1 e2 e3) (IfE e1' e2 e3)
+    .
+
+End Reduction_Semantics.
+
+
+(* ~~~~~~~~~~~~~~~~~~~~~~~~~~~~~~~~~~~~~~~~~~~~~~~~~~~~~~~~~~ *)
+Section Type_System.
+Open Scope exp_scope. (* need to reopen since the old section was closed *)
+
+(* notation for [FunT] was (infix "\<rightarrow>" 75) *)
+Inductive ty := 
+    | IntT  : ty
+    | BoolT : ty
+    | FunT  : ty -> ty -> ty
+    .
+
+(* Personally, I'd return [FunT t1 t2] everywhere instead of [(t1,t2)]... *)
+Definition prim_type (p:primitive) : ty * ty :=
+    match p with
+    | Inc    => (IntT,  IntT)
+    | Dec    => (IntT,  IntT)
+    | Neg    => (IntT,  IntT)
+    | IsZero => (IntT,  BoolT)
+    | Not    => (BoolT, BoolT)
+    end.
+
+Definition const_type (c:const) : ty :=
+    match c with
+    | IntC  _ => IntT
+    | BoolC _ => BoolT
+    end.
+
+
+(* See LNVarMap.v for the definitions of [lookup], [lookup_app], [lookup_app_none], [not_dom_lookup_none], [lookup_dom] *)
+
+Definition ty_env := VarMap Var ty.
+Implicit Type Γ : ty_env.
+
+
+Inductive wt : ty_env -> exp -> ty -> Prop :=
+    | wt_c
+        : forall Γ c T
+        ,  const_type c = T
+        -> wt Γ (Const c) T
+    | wt_p
+        : forall Γ p e T1 T2
+        ,  wt Γ e T1
+        -> prim_type p = (T1, T2)
+        -> wt Γ (Prim p e) T2
+    | wt_i
+        : forall Γ e1 e2 e3 T
+        ,  wt Γ e1 BoolT
+        -> wt Γ e2 T
+        -> wt Γ e3 T
+        -> wt Γ (IfE e1 e2 e3) T
+    | wt_v
+        : forall Γ x T
+        ,  lookup x Γ = Some T
+        -> wt Γ (FVar x) T
+    | wt_l
+        : forall Γ e x T1 T2
+        ,  x \freshin e
+        -> wt ((x,T1)::Γ) (∆x·e) T2
+        -> wt Γ (LambdaE e) (FunT T1 T2)
+    | wt_a
+        : forall Γ e1 e2 T T'
+        ,  wt Γ e1 (FunT T T')
+        -> wt Γ e2 T
+        -> wt Γ (AppE e1 e2) T'
+    .
+(* Notation was ("_ \<turnstile>o _ : _" [60,60,60] 59) *)
+(* Technically we should use [⊦] instead of [⊢] *)
+Notation "Γ ⊢o e : T" := (wt Γ e T)
+    (at level 0, e at level 99, no associativity) :type_scope.
+
 (*
-lemma interp_mono: assumes ie: "interp e n = Res v'" and nn: "n \<le> n'" 
-  shows "interp e n' = Res v'"
-  using ie nn apply (induction e n arbitrary: v' n' rule: interp.induct)
-  apply (case_tac n') apply simp apply force
-  apply (case_tac n') apply force apply (case_tac "interp e n") apply force 
-      apply force apply force
-  apply (erule inv_interp_if) apply (case_tac n') apply force
-    apply (case_tac b) apply force apply force 
-  apply simp
-  apply simp
-  apply (case_tac n') apply simp apply force 
-  apply (erule inv_interp_app) apply (case_tac n') apply force apply force
-  apply simp
-done
-
-
-section "Reduction Semantics"
-
-primrec close :: "nat \<Rightarrow> var \<Rightarrow> exp \<Rightarrow> exp" ("{_\<leftarrow>_}_" [54,54,54] 53) where
-  "{j\<leftarrow>x} (Const c) = Const c" |
-  "{j\<leftarrow>x} (Prim p e') = Prim p ({j\<leftarrow>x} e')" |
-  "{j\<leftarrow>x} (IfE e1 e2 e3) = IfE ({j\<leftarrow>x} e1) ({j\<leftarrow>x} e2) ({j\<leftarrow>x} e3)" |
-  "{j\<leftarrow>x} (FVar y) = (if x = y then BVar j else FVar y)" |
-  "{j\<leftarrow>x} (BVar k) = BVar k" |
-  "{j\<leftarrow>x} (LambdaE e') = LambdaE ({(Suc j)\<leftarrow>x} e')" |
-  "{j\<leftarrow>x} (AppE e1 e2) = AppE ({j\<leftarrow>x} e1) ({j\<leftarrow>x} e2)"
-
-
-inductive reduce_fb :: "exp \<Rightarrow> exp \<Rightarrow> bool" (infix "\<longmapsto>fb" 70) where
-  full_beta[intro!]: "AppE (LambdaE e) e' \<longmapsto>fb ({0\<rightarrow>e'}e)" |
-  c_lambda[intro!]: "\<lbrakk> x \<notin> set (FV e); ({0\<rightarrow>FVar x}e) \<longmapsto>fb e' \<rbrakk>
-                     \<Longrightarrow> (LambdaE e) \<longmapsto>fb (LambdaE ({0\<leftarrow>x}e'))" |
-  c_app1_fb[intro!]: "\<lbrakk> e1 \<longmapsto>fb e1' \<rbrakk> \<Longrightarrow> AppE e1 e2 \<longmapsto>fb AppE e1' e2" |
-  c_app2_fb[intro!]: "\<lbrakk> e2 \<longmapsto>fb e2' \<rbrakk> \<Longrightarrow> AppE e1 e2 \<longmapsto>fb AppE e1 e2'" |
-  r_prim_fb[intro!]: "\<lbrakk> eval_prim p c = Result c' \<rbrakk>
-                     \<Longrightarrow> Prim p (Const c) \<longmapsto>fb Const c'" |
-  c_prim_fb[intro!]: "\<lbrakk> e \<longmapsto>fb e' \<rbrakk> \<Longrightarrow> Prim p e \<longmapsto>fb Prim p e'" |
-  r_if_true_fb[intro!]: "IfE (Const (BoolC True)) e2 e3 \<longmapsto>fb e2" |
-  r_if_false_fb[intro!]: "IfE (Const (BoolC False)) e2 e3 \<longmapsto>fb e3" |
-  c_if1_fb[intro!]: "\<lbrakk> e1 \<longmapsto>fb e1' \<rbrakk> \<Longrightarrow> IfE e1 e2 e3 \<longmapsto>fb IfE e1' e2 e3" |
-  c_if2_fb[intro!]: "\<lbrakk> e2 \<longmapsto>fb e2' \<rbrakk> \<Longrightarrow> IfE e1 e2 e3 \<longmapsto>fb IfE e1 e2' e3" |
-  c_if3_fb[intro!]: "\<lbrakk> e3 \<longmapsto>fb e3' \<rbrakk> \<Longrightarrow> IfE e1 e2 e3 \<longmapsto>fb IfE e1 e2 e3'" 
-
-
-fun val :: "exp \<Rightarrow> bool" where
-  "val (Const c) = True" |
-  "val (LambdaE e) = True" |
-  "val _ = False" 
-
-inductive reduce_bv :: "exp \<Rightarrow> exp \<Rightarrow> bool" (infix "\<longmapsto>" 70) where
-  beta_bv[intro!]: "val v \<Longrightarrow> AppE (LambdaE e) v \<longmapsto> ({0\<rightarrow>v}e)" |
-  c_app1_bv[intro!]: "\<lbrakk> e1 \<longmapsto> e1' \<rbrakk> \<Longrightarrow> AppE e1 e2 \<longmapsto> AppE e1' e2" |
-  c_app2_bv[intro!]: "\<lbrakk> val v; e2 \<longmapsto> e2' \<rbrakk> \<Longrightarrow> AppE v e2 \<longmapsto> AppE v e2'" |
-  r_prim_bv[intro!]: "\<lbrakk> eval_prim p c = Result c' \<rbrakk>
-                     \<Longrightarrow> Prim p (Const c) \<longmapsto> Const c'" |
-  c_prim_bv[intro!]: "\<lbrakk> e \<longmapsto> e' \<rbrakk> \<Longrightarrow> Prim p e \<longmapsto> Prim p e'" |
-  r_if_true_bv[intro!]: "IfE (Const (BoolC True)) e2 e3 \<longmapsto> e2" |
-  r_if_false_bv[intro!]: "IfE (Const (BoolC False)) e2 e3 \<longmapsto> e3" |
-  c_if_bv[intro!]: "\<lbrakk> e1 \<longmapsto> e1' \<rbrakk> \<Longrightarrow> IfE e1 e2 e3 \<longmapsto> IfE e1' e2 e3" 
-
-inductive reduces_bv :: "exp \<Rightarrow> exp \<Rightarrow> bool" (infix "\<longmapsto>*" 70) where
- red_bv_nil[intro!]: "(e::exp) \<longmapsto>* e" |
- red_bv_cons[intro!]: "\<lbrakk> (e1::exp) \<longmapsto> e2; e2 \<longmapsto>* e3 \<rbrakk> \<Longrightarrow> e1 \<longmapsto>* e3"
-
-
-inductive reduce_bn :: "exp \<Rightarrow> exp \<Rightarrow> bool" (infix "\<longmapsto>bn" 70) where
-  beta_bn[intro!]: "AppE (LambdaE e) e' \<longmapsto>bn ({0\<rightarrow>e'}e)" |
-  c_app_bn[intro!]: "\<lbrakk> e1 \<longmapsto>bn e1' \<rbrakk> \<Longrightarrow> AppE e1 e2 \<longmapsto>bn AppE e1' e2" |
-  r_prim_bn[intro!]: "\<lbrakk> eval_prim p c = Result c' \<rbrakk>
-                     \<Longrightarrow> Prim p (Const c) \<longmapsto>bn Const c'" |
-  c_prim_bn[intro!]: "\<lbrakk> e \<longmapsto>bn e' \<rbrakk> \<Longrightarrow> Prim p e \<longmapsto>bn Prim p e'" |
-  r_if_true_bn[intro!]: "IfE (Const (BoolC True)) e2 e3 \<longmapsto>bn e2" |
-  r_if_false_bn[intro!]: "IfE (Const (BoolC False)) e2 e3 \<longmapsto>bn e3" |
-  c_if_bn[intro!]: "\<lbrakk> e1 \<longmapsto>bn e1' \<rbrakk> \<Longrightarrow> IfE e1 e2 e3 \<longmapsto>bn IfE e1' e2 e3"
-
-
-
-section "Type System"
-
-
-datatype ty = IntT | BoolT | FunT ty ty (infix "\<rightarrow>" 75)
-
-
-primrec prim_type :: "primitive \<Rightarrow> ty \<times> ty" where
-   "prim_type Inc = (IntT, IntT)" |
-   "prim_type Dec = (IntT, IntT)" |
-   "prim_type Neg = (IntT, IntT)" |
-   "prim_type IsZero = (IntT, BoolT)" |
-   "prim_type Not = (BoolT, BoolT)" 
-
-primrec const_type :: "const \<Rightarrow> ty" where
-  "const_type (IntC n) = IntT" |
-  "const_type (BoolC b) = BoolT"
-
-fun lookup :: "'a \<Rightarrow> ('a \<times> 'b) list \<Rightarrow> 'b option" where
-  "lookup k [] = None" |
-  "lookup k ((k',v)#ls) = (if k = k' then Some v else lookup k ls)"
-
-
-lemma lookup_app: assumes lx: "lookup x \<Gamma> = Some v" 
-  shows "lookup x (\<Gamma>@\<Gamma>') = Some v"
-  using lx by (induction \<Gamma> arbitrary: x v) auto 
-
-lemma lookup_app_none: assumes lx: "lookup x \<Gamma> = None" 
-  shows "lookup x (\<Gamma>@[(x,T)]) = Some T"
-  using lx by (induction \<Gamma> arbitrary: x T) auto
-
-lemma not_dom_lookup_none: 
-  assumes x: "x \<notin> assoc_dom \<Gamma>" shows "lookup x \<Gamma> = None"
-  using x by (induction \<Gamma> arbitrary: x) auto
-
-lemma lookup_dom: 
-  assumes x: "lookup x \<Gamma> = Some T" shows "x \<in> assoc_dom \<Gamma>"
-  using x apply (induction \<Gamma> arbitrary: x T) apply auto 
-  apply (case_tac "x = a") by auto 
-
-type_synonym ty_env = "(var \<times> ty) list"
-
-
-inductive wt :: "ty_env \<Rightarrow> exp \<Rightarrow> ty \<Rightarrow> bool" ("_ \<turnstile>o _ : _" [60,60,60] 59) where
-  wt_c[intro!]: "\<lbrakk> const_type c = T \<rbrakk> \<Longrightarrow> \<Gamma> \<turnstile>o Const c : T" |
-  wt_p[intro!]: "\<lbrakk> \<Gamma> \<turnstile>o e : T1; prim_type p = (T1, T2) \<rbrakk>
-          \<Longrightarrow> \<Gamma> \<turnstile>o Prim p e : T2" |
-  wt_i[intro!]: "\<lbrakk> \<Gamma> \<turnstile>o e1 : BoolT; \<Gamma> \<turnstile>o e2 : T; \<Gamma> \<turnstile>o e3 : T \<rbrakk> 
-                    \<Longrightarrow> \<Gamma> \<turnstile>o IfE e1 e2 e3 : T" |
-  wt_v[intro!]: "\<lbrakk> lookup x \<Gamma> = Some T \<rbrakk> \<Longrightarrow> \<Gamma> \<turnstile>o FVar x : T" |
-  wt_l[intro!]: "\<lbrakk> x \<notin> set (FV e); (x,T1)#\<Gamma> \<turnstile>o ({0\<rightarrow>FVar x} e) : T2 \<rbrakk> 
-          \<Longrightarrow> \<Gamma> \<turnstile>o LambdaE e : T1\<rightarrow>T2" |
-  wt_a[intro!]: "\<lbrakk> \<Gamma> \<turnstile>o e1 : T \<rightarrow> T'; \<Gamma> \<turnstile>o e2 : T \<rbrakk> 
-          \<Longrightarrow> \<Gamma> \<turnstile>o AppE e1 e2 : T'"
-
-
-inductive well_typed :: "ty_env \<Rightarrow> exp \<Rightarrow> ty \<Rightarrow> bool" ("_ \<turnstile> _ : _" [60,60,60] 59) where
-  wt_const[intro!]: "\<lbrakk> const_type c = T \<rbrakk> \<Longrightarrow> \<Gamma> \<turnstile> Const c : T" |
-  wt_prim[intro!]: "\<lbrakk> \<Gamma> \<turnstile> e : T1; prim_type p = (T1, T2) \<rbrakk>
-          \<Longrightarrow> \<Gamma> \<turnstile> Prim p e : T2" |
-  wt_if[intro!]: "\<lbrakk> \<Gamma> \<turnstile> e1 : BoolT; \<Gamma> \<turnstile> e2 : T; \<Gamma> \<turnstile> e3 : T \<rbrakk> 
-                    \<Longrightarrow> \<Gamma> \<turnstile> IfE e1 e2 e3 : T" |
-  wt_var[intro!]: "\<lbrakk> lookup x \<Gamma> = Some T \<rbrakk> \<Longrightarrow> \<Gamma> \<turnstile> FVar x : T" |
-  wt_lambda[intro!]: "\<lbrakk> \<forall> x. x \<notin> set L \<longrightarrow> (x,T1)#\<Gamma> \<turnstile> ({0\<rightarrow>FVar x} e) : T2 \<rbrakk> 
-          \<Longrightarrow> \<Gamma> \<turnstile> LambdaE e : T1\<rightarrow>T2" |
-  wt_app[intro!]: "\<lbrakk> \<Gamma> \<turnstile> e1 : T \<rightarrow> T'; \<Gamma> \<turnstile> e2 : T \<rbrakk> 
-          \<Longrightarrow> \<Gamma> \<turnstile> AppE e1 e2 : T'"
+inductive well_typed :: "ty_env => exp => ty => bool" ("_ ⊢ _ : _" [60,60,60] 59) where
+  wt_const : "[| const_type c = T |] ==> Γ ⊢ Const c : T" |
+  wt_prim : "[| Γ ⊢ e : T1; prim_type p = (T1, T2) |]
+          ==> Γ ⊢ Prim p e : T2" |
+  wt_if : "[| Γ ⊢ e1 : BoolT; Γ ⊢ e2 : T; Γ ⊢ e3 : T |] 
+                    ==> Γ ⊢ IfE e1 e2 e3 : T" |
+  wt_var : "[| lookup x Γ = Some T |] ==> Γ ⊢ FVar x : T" |
+  wt_lambda : "[| \<forall> x. x \<notin> set L \<longrightarrow> (x,T1)::Γ ⊢ (∆x·e) : T2 |] 
+          ==> Γ ⊢ LambdaE e : T1\<rightarrow>T2" |
+  wt_app : "[| Γ ⊢ e1 : T \<rightarrow> T'; Γ ⊢ e2 : T |] 
+          ==> Γ ⊢ AppE e1 e2 : T'"
 
 inductive_cases
-  inv_wt_fvar[elim!]: "\<Gamma> \<turnstile> FVar x : T" and
-  inv_wt_bvar[elim!]: "\<Gamma> \<turnstile> BVar k : T" and
-  inv_wt_const[elim!]: "\<Gamma> \<turnstile> Const c : T" and
-  inv_wt_prim[elim!]: "\<Gamma> \<turnstile> Prim p e : T" and
-  inv_wt_lambda[elim!]: "\<Gamma> \<turnstile> LambdaE e : T" and
-  inv_wt_app[elim!]: "\<Gamma> \<turnstile> AppE e1 e2 : T"
+  inv_wt_fvar[elim!]: "Γ ⊢ FVar x : T" and
+  inv_wt_bvar[elim!]: "Γ ⊢ BVar k : T" and
+  inv_wt_const[elim!]: "Γ ⊢ Const c : T" and
+  inv_wt_prim[elim!]: "Γ ⊢ Prim p e : T" and
+  inv_wt_lambda[elim!]: "Γ ⊢ LambdaE e : T" and
+  inv_wt_app[elim!]: "Γ ⊢ AppE e1 e2 : T"
 
 
-inductive wt_env :: "ty_env \<Rightarrow> env \<Rightarrow> bool" ("_ \<turnstile> _" [60,60] 59) where
-wt_nil[intro!]: "[] \<turnstile> []" |
-wt_cons[intro!]: "\<lbrakk> [] \<turnstile> v : T; \<Gamma> \<turnstile> \<rho> \<rbrakk> \<Longrightarrow> (x,T)#\<Gamma> \<turnstile> (x,v)#\<rho>"
+inductive wt_env :: "ty_env => env => bool" ("_ ⊢ _" [60,60] 59) where
+wt_nil : "[] ⊢ []" |
+wt_cons : "[| [] ⊢ v : T; Γ ⊢ ρ |] ==> (x,T)::Γ ⊢ (x,v)::ρ"
 
 inductive_cases
-  inv_wt_nil[elim!]: "\<Gamma> \<turnstile> []" and
-  inv_wt_cons[elim!]: "\<Gamma> \<turnstile> (x,v)#\<rho>"
+  inv_wt_nil[elim!]: "Γ ⊢ []" and
+  inv_wt_cons[elim!]: "Γ ⊢ (x,v)::ρ"
 
 
 section "Properties of Substitution" 
@@ -658,8 +751,8 @@ lemma bsubst_cross[rule_format]:
   done
 
 
-lemma bsubst_id: fixes e::exp assumes wte: "\<Gamma> \<turnstile> e : T" shows "{k\<rightarrow>e'}e = e"
-  using wte apply (induction \<Gamma> e T arbitrary: k e')
+lemma bsubst_id: fixes e::exp assumes wte: "Γ ⊢ e : T" shows "{k\<rightarrow>e'}e = e"
+  using wte apply (induction Γ e T arbitrary: k e')
   apply force apply force apply force apply force defer apply force
   apply (erule_tac x="Suc (list_max L)" in allE) apply (erule impE) 
   apply (rule list_max_fresh) apply simp apply simp apply clarify 
@@ -673,9 +766,9 @@ lemma fv_bsubst: fixes e::exp and e'::exp shows "set (FV e) \<subseteq> set (FV 
 
 lemma subst_permute:
   fixes x::nat and z::nat and e::exp and e'::exp
-  assumes xz: "z \<notin> set (FV v)" and wte: "\<Gamma> \<turnstile> e' : T"
-  shows "{j\<rightarrow>v}([z\<mapsto>e']e) = [z\<mapsto>e']({j\<rightarrow>v}e)"
-  using xz wte apply (induction e arbitrary: j x z \<Gamma> T e') 
+  assumes xz: "z \<notin> set (FV v)" and wte: "Γ ⊢ e' : T"
+  shows "{j\<rightarrow>v}([[z~>e']]e) = [[z~>e']]({j\<rightarrow>v}e)"
+  using xz wte apply (induction e arbitrary: j x z Γ T e') 
   apply force apply force apply force
   using bsubst_id apply force apply simp
   using subst_id apply force apply force apply force 
@@ -683,7 +776,7 @@ lemma subst_permute:
 
 
 lemma decompose_subst[rule_format]:
-  "\<forall> u x i. x \<notin> set (FV e) \<longrightarrow> {i\<rightarrow>u}e = [x\<mapsto>u]({i\<rightarrow>FVar x}e)"
+  "\<forall> u x i. x \<notin> set (FV e) \<longrightarrow> {i\<rightarrow>u}e = [[x~>u]]({i\<rightarrow>FVar x}e)"
   apply (induction e)
   apply force
   apply clarify apply (erule_tac x=u in allE) apply (erule_tac x=x in allE) 
@@ -698,54 +791,54 @@ lemma decompose_subst[rule_format]:
 section "Properties of Multiple Substitutions"
 
 
-lemma msubst_const[simp]: "[\<rho>]Const c = Const c" by (induction \<rho>) auto
+lemma msubst_const[simp]: "[ρ]Const c = Const c" by (induction ρ) auto
 
-lemma msubst_prim[simp]: "[\<rho>]Prim p e = Prim p ([\<rho>]e)"
-  by (induction \<rho> arbitrary: p e) auto
+lemma msubst_prim[simp]: "[ρ]Prim p e = Prim p ([ρ]e)"
+  by (induction ρ arbitrary: p e) auto
 
-lemma msubst_var1: fixes v::exp assumes lx: "lookup x \<rho> = Some v" and fv: "FV v = []" 
-  shows "[\<rho>]FVar x = v"
-  using lx fv apply (induction \<rho> arbitrary: x v)
+lemma msubst_var1: fixes v::exp assumes lx: "lookup x ρ = Some v" and fv: "FV v = []" 
+  shows "[ρ]FVar x = v"
+  using lx fv apply (induction ρ arbitrary: x v)
   apply force
   apply (case_tac a) apply simp apply (case_tac "x = aa")
   apply simp apply (rule msubst_id) apply auto
   done
   
 lemma msubst_var2:
-  fixes v::exp assumes lx: "lookup x \<rho> = None" shows "[\<rho>]FVar x = FVar x"
-  using lx by (induction \<rho> arbitrary: x v) auto
+  fixes v::exp assumes lx: "lookup x ρ = None" shows "[ρ]FVar x = FVar x"
+  using lx by (induction ρ arbitrary: x v) auto
 
-lemma msubst_if[simp]: "[\<rho>]IfE e1 e2 e3 = IfE ([\<rho>]e1) ([\<rho>]e2) ([\<rho>]e3)"
-  by (induction \<rho> arbitrary: e1 e2 e3) auto 
+lemma msubst_if[simp]: "[ρ]IfE e1 e2 e3 = IfE ([ρ]e1) ([ρ]e2) ([ρ]e3)"
+  by (induction ρ arbitrary: e1 e2 e3) auto 
 
-lemma msubst_app[simp]: "[\<rho>]AppE e1 e2 = AppE ([\<rho>]e1) ([\<rho>]e2)"
-  by (induction \<rho> arbitrary: e1 e2) auto
+lemma msubst_app[simp]: "[ρ]AppE e1 e2 = AppE ([ρ]e1) ([ρ]e2)"
+  by (induction ρ arbitrary: e1 e2) auto
 
-lemma msubst_lam[simp]: "[\<rho>]LambdaE e = LambdaE ([\<rho>]e)"
-  by (induction \<rho> arbitrary: e) auto
+lemma msubst_lam[simp]: "[ρ]LambdaE e = LambdaE ([ρ]e)"
+  by (induction ρ arbitrary: e) auto
 
 lemma msubst_permute:
-  fixes e::exp and \<rho>::env
-  assumes rv: "assoc_dom \<rho> \<inter> set (FV v) = {}" and wtr: "\<Gamma> \<turnstile> \<rho>"
-  shows "{j\<rightarrow>v}([\<rho>]e) = [\<rho>]({j\<rightarrow>v}e)"
-using rv wtr proof (induction \<rho> arbitrary: j v e \<Gamma>)
+  fixes e::exp and ρ::env
+  assumes rv: "assoc_dom ρ \<inter> set (FV v) = {}" and wtr: "Γ ⊢ ρ"
+  shows "{j\<rightarrow>v}([ρ]e) = [ρ]({j\<rightarrow>v}e)"
+using rv wtr proof (induction ρ arbitrary: j v e Γ)
   case (Nil j v e)
   show "{j\<rightarrow>v}[[]] e = [[]]({j\<rightarrow>v}e)" by simp
 next
-  case (Cons a \<rho> j v e)
-  show "{j\<rightarrow>v}[(a # \<rho>)] e = [(a # \<rho>)] ({j\<rightarrow>v}e)"
+  case (Cons a ρ j v e)
+  show "{j\<rightarrow>v}[(a :: ρ)] e = [(a :: ρ)] ({j\<rightarrow>v}e)"
   proof (cases a)
     fix z e' assume a: "a = (z,e')"
-    let ?E = "[z\<mapsto>e']e"
-    from a have "[(a # \<rho>)] e = [\<rho>]( ?E )" by simp
-    from Cons have d: "assoc_dom \<rho> \<inter> set (FV v) = {}" by auto
-    from Cons a obtain \<Gamma>' T where g: "\<Gamma> = (z,T)#\<Gamma>'" and gr2: "\<Gamma>' \<turnstile> \<rho>" 
-      and wtep: "[] \<turnstile> e' : T" by blast
+    let ?E = "[[z~>e']]e"
+    from a have "[(a :: ρ)] e = [ρ]( ?E )" by simp
+    from Cons have d: "assoc_dom ρ \<inter> set (FV v) = {}" by auto
+    from Cons a obtain Γ' T where g: "Γ = (z,T)::Γ'" and gr2: "Γ' ⊢ ρ" 
+      and wtep: "[] ⊢ e' : T" by blast
     from Cons a have zfv: "z \<notin> set (FV v)" by simp
-    from Cons a d gr2 have IH: "{j\<rightarrow>v}[\<rho>] ?E = [\<rho>]({j\<rightarrow>v} ?E)" by blast
-    also with zfv wtep have "... = [\<rho>]([z\<mapsto>e']({j\<rightarrow>v}e))"
+    from Cons a d gr2 have IH: "{j\<rightarrow>v}[ρ] ?E = [ρ]({j\<rightarrow>v} ?E)" by blast
+    also with zfv wtep have "... = [ρ]([[z~>e']]({j\<rightarrow>v}e))"
       using subst_permute[of z v "[]" e' T j e] by simp
-    finally have "{j\<rightarrow>v}[\<rho>] ([z\<mapsto>e']e) = [\<rho>]([z\<mapsto>e']({j\<rightarrow>v}e))" by simp
+    finally have "{j\<rightarrow>v}[ρ] ([[z~>e']]e) = [ρ]([[z~>e']]({j\<rightarrow>v}e))" by simp
     with a show ?thesis by simp
   qed
 qed
@@ -754,23 +847,23 @@ qed
 section "Properties of Environments"
 
 lemma wt_env_lookup:
-  assumes lg: "lookup x \<Gamma> = Some T" and wt_env: "\<Gamma> \<turnstile> \<rho>"
-  shows "\<exists> (v::exp). lookup x \<rho> = Some v \<and> [] \<turnstile> v : T"
-  using wt_env lg by (induction \<Gamma> \<rho> arbitrary: x T) auto
+  assumes lg: "lookup x Γ = Some T" and wt_env: "Γ ⊢ ρ"
+  shows "\<exists> (v::exp). lookup x ρ = Some v \<and> [] ⊢ v : T"
+  using wt_env lg by (induction Γ ρ arbitrary: x T) auto
 
-abbreviation subseteq :: "ty_env \<Rightarrow> ty_env \<Rightarrow> bool" (infixl "\<preceq>" 80) where
-  "\<Gamma> \<preceq> \<Gamma>' \<equiv> \<forall> x T. lookup x \<Gamma> = Some T \<longrightarrow> lookup x \<Gamma>' = Some T"
+abbreviation subseteq :: "ty_env => ty_env => bool" (infixl "\<preceq>" 80) where
+  "Γ \<preceq> Γ' \<equiv> \<forall> x T. lookup x Γ = Some T \<longrightarrow> lookup x Γ' = Some T"
 
 lemma env_weakening[rule_format]:
-  fixes e::exp shows "\<Gamma> \<turnstile> e : T \<Longrightarrow> \<forall> \<Gamma>'. \<Gamma> \<preceq> \<Gamma>' \<longrightarrow> \<Gamma>' \<turnstile> e : T" 
+  fixes e::exp shows "Γ ⊢ e : T ==> \<forall> Γ'. Γ \<preceq> Γ' \<longrightarrow> Γ' ⊢ e : T" 
   apply (induct rule: well_typed.induct)
   apply force
-  apply (rule allI) apply (rule impI) apply (erule_tac x=\<Gamma>' in allE) apply force
+  apply (rule allI) apply (rule impI) apply (erule_tac x=Γ' in allE) apply force
   apply force
   apply force
   defer
-  apply (rule allI) apply (rule impI) apply (erule_tac x=\<Gamma>' in allE) 
-    apply (erule_tac x=\<Gamma>' in allE) apply simp apply blast
+  apply (rule allI) apply (rule impI) apply (erule_tac x=Γ' in allE) 
+    apply (erule_tac x=Γ' in allE) apply simp apply blast
   apply (rule allI) apply (rule impI)
   apply (rule wt_lambda) apply (rule allI) apply (rule impI)
   apply (erule_tac x=x in allE) apply (erule impE) apply assumption
@@ -778,8 +871,8 @@ lemma env_weakening[rule_format]:
 done
 
 lemma wt_dom_fv: 
-  assumes wt: "\<Gamma> \<turnstile>o e : T" shows "set (FV e) \<subseteq> assoc_dom \<Gamma>"
-  using wt apply (induction \<Gamma> e T)
+  assumes wt: "Γ ⊢o e : T" shows "set (FV e) \<subseteq> assoc_dom Γ"
+  using wt apply (induction Γ e T)
   apply simp
   apply force
   apply force
@@ -789,114 +882,114 @@ lemma wt_dom_fv:
   using fv_bsubst apply force
   done
 
-lemma weaken_cons_snoc: assumes xng: "x \<notin> assoc_dom \<Gamma>" 
-  shows "([(x,T1)]@\<Gamma>) \<preceq> (\<Gamma>@[(x,T1)])" using xng
+lemma weaken_cons_snoc: assumes xng: "x \<notin> assoc_dom Γ" 
+  shows "([(x,T1)]++Γ) \<preceq> (Γ++[(x,T1)])" using xng
 proof clarify
-  fix x' T assume lxg1: "lookup x' ([(x,T1)]@\<Gamma>) = Some T"
-  show "lookup x' (\<Gamma>@[(x,T1)]) = Some T"
+  fix x' T assume lxg1: "lookup x' ([(x,T1)]++Γ) = Some T"
+  show "lookup x' (Γ++[(x,T1)]) = Some T"
   proof (cases "x' = x")
     assume x: "x' = x"
-    with lxg1 have lxg1b: "lookup x' ([(x,T1)]@\<Gamma>) = Some T1" by simp
-    from xng not_dom_lookup_none have xg: "lookup x \<Gamma> = None" by simp
-    from lxg1b xg x have "lookup x' (\<Gamma>@[(x,T1)]) = Some T1"
-      using lookup_app_none[of x \<Gamma>] by simp
+    with lxg1 have lxg1b: "lookup x' ([(x,T1)]++Γ) = Some T1" by simp
+    from xng not_dom_lookup_none have xg: "lookup x Γ = None" by simp
+    from lxg1b xg x have "lookup x' (Γ++[(x,T1)]) = Some T1"
+      using lookup_app_none[of x Γ] by simp
     with x lxg1 show ?thesis by simp
   next
     assume x: "x' \<noteq> x"
-    from x lxg1 have lxg1b: "lookup x' \<Gamma> = Some T" by simp
+    from x lxg1 have lxg1b: "lookup x' Γ = Some T" by simp
     thus ?thesis by (rule lookup_app)
   qed
 qed
 
 section "Substitution Preserves Types"
 
-abbreviation remove_bind :: "var \<Rightarrow> ty_env \<Rightarrow> ty_env \<Rightarrow> bool" where
-  "remove_bind z \<Gamma> \<Gamma>' \<equiv> \<forall>x T. x\<noteq>z \<and> lookup x \<Gamma> = Some T 
-            \<longrightarrow> lookup x \<Gamma>' = Some T"
+abbreviation remove_bind :: "var => ty_env => ty_env => bool" where
+  "remove_bind z Γ Γ' \<equiv> \<forall>x T. x\<noteq>z \<and> lookup x Γ = Some T 
+            \<longrightarrow> lookup x Γ' = Some T"
 
 lemma subst_pres_types:
-  fixes M::exp and v::exp and \<Gamma>::ty_env
-  assumes wtm: "\<Gamma> \<turnstile> M : A" and lx: "lookup x \<Gamma> = Some B"
-  and rg: "remove_bind x \<Gamma> \<Gamma>'" and vb: "\<Gamma>' \<turnstile> v : B"
-  shows "\<Gamma>' \<turnstile> [x \<mapsto> v]M : A" using wtm lx rg vb
-proof (induction arbitrary: x B \<Gamma>' v rule: well_typed.induct)
-  case (wt_const c T \<Gamma> x B \<Gamma>' v)
-  thus "\<Gamma>' \<turnstile> [x\<mapsto>v](Const c) : T" by auto
+  fixes M::exp and v::exp and Γ::ty_env
+  assumes wtm: "Γ ⊢ M : A" and lx: "lookup x Γ = Some B"
+  and rg: "remove_bind x Γ Γ'" and vb: "Γ' ⊢ v : B"
+  shows "Γ' ⊢ [[x~>v]]M : A" using wtm lx rg vb
+proof (induction arbitrary: x B Γ' v rule: well_typed.induct)
+  case (wt_const c T Γ x B Γ' v)
+  thus "Γ' ⊢ [[x~>v]](Const c) : T" by auto
 next
-  case (wt_prim \<Gamma> e T1 p T2 x B \<Gamma>' v)
-  hence "\<Gamma>' \<turnstile> [x\<mapsto>v]e : T1" and "prim_type p = (T1,T2)" by auto
-  thus "\<Gamma>' \<turnstile> [x\<mapsto>v] (Prim p e) : T2" by auto
+  case (wt_prim Γ e T1 p T2 x B Γ' v)
+  hence "Γ' ⊢ [[x~>v]]e : T1" and "prim_type p = (T1,T2)" by auto
+  thus "Γ' ⊢ [[x~>v]] (Prim p e) : T2" by auto
 next
-  case (wt_if \<Gamma> e1 e2 T e3 x B \<Gamma>' v)
-  from wt_if have wte1: "\<Gamma>' \<turnstile> [x\<mapsto>v]e1 : BoolT" 
-    and wte2: "\<Gamma>' \<turnstile> [x\<mapsto>v]e2 : T"  and wte3: "\<Gamma>' \<turnstile> [x\<mapsto>v]e3 : T" by auto
-  from wte1 wte2 wte3 show "\<Gamma>' \<turnstile> [x\<mapsto>v] IfE e1 e2 e3 : T" by auto
+  case (wt_if Γ e1 e2 T e3 x B Γ' v)
+  from wt_if have wte1: "Γ' ⊢ [[x~>v]]e1 : BoolT" 
+    and wte2: "Γ' ⊢ [[x~>v]]e2 : T"  and wte3: "Γ' ⊢ [[x~>v]]e3 : T" by auto
+  from wte1 wte2 wte3 show "Γ' ⊢ [[x~>v]] IfE e1 e2 e3 : T" by auto
 next
-  case (wt_var y \<Gamma> T x B \<Gamma>' v)
-  from wt_var have wtv: "\<Gamma>' \<turnstile> v : B" and ly: "lookup y \<Gamma> = Some T" 
-      and lx: "lookup x \<Gamma> = Some B" and rb: "remove_bind x \<Gamma> \<Gamma>'" by auto
-  show "\<Gamma>' \<turnstile> [x\<mapsto>v]FVar y : T"
+  case (wt_var y Γ T x B Γ' v)
+  from wt_var have wtv: "Γ' ⊢ v : B" and ly: "lookup y Γ = Some T" 
+      and lx: "lookup x Γ = Some B" and rb: "remove_bind x Γ Γ'" by auto
+  show "Γ' ⊢ [[x~>v]]FVar y : T"
   proof (cases "x = y")
     assume x: "x = y"
-    have "[] \<preceq> \<Gamma>'" by auto
+    have "[] \<preceq> Γ'" by auto
     from wtv x ly lx show ?thesis by simp
   next
-    assume x: "x \<noteq> y" with ly rb have "\<Gamma>' \<turnstile> FVar y : T" by auto
+    assume x: "x \<noteq> y" with ly rb have "Γ' ⊢ FVar y : T" by auto
     with x show ?thesis by auto
   qed
 next
-  case (wt_lambda L T1 \<Gamma> e T2 x B \<Gamma>' v)
-  from wt_lambda have lx: "lookup x \<Gamma> = Some B" by simp
-  from wt_lambda have rb: "remove_bind x \<Gamma> \<Gamma>'" by simp
-  from wt_lambda have wtv: "\<Gamma>' \<turnstile> v : B" by simp
-  have "\<Gamma>' \<turnstile> LambdaE ([x\<mapsto>v]e) : T1 \<rightarrow> T2"
+  case (wt_lambda L T1 Γ e T2 x B Γ' v)
+  from wt_lambda have lx: "lookup x Γ = Some B" by simp
+  from wt_lambda have rb: "remove_bind x Γ Γ'" by simp
+  from wt_lambda have wtv: "Γ' ⊢ v : B" by simp
+  have "Γ' ⊢ LambdaE ([[x~>v]]e) : T1 \<rightarrow> T2"
   proof clarify
-    fix x' assume xL: "x' \<notin> set ((x#L) @ (map fst \<Gamma>'))"
-    from wt_lambda xL have "(x',T1)#\<Gamma> \<turnstile> bsubst 0 (FVar x') e : T2" by auto
-    from xL lx have lx2: "lookup x ((x',T1)#\<Gamma>) = Some B" by simp
-    from rb xL have rb2: "remove_bind x ((x',T1)#\<Gamma>) ((x',T1)#\<Gamma>')" by auto
+    fix x' assume xL: "x' \<notin> set ((x::L) ++ (map fst Γ'))"
+    from wt_lambda xL have "(x',T1)::Γ ⊢ bsubst 0 (FVar x') e : T2" by auto
+    from xL lx have lx2: "lookup x ((x',T1)::Γ) = Some B" by simp
+    from rb xL have rb2: "remove_bind x ((x',T1)::Γ) ((x',T1)::Γ')" by auto
     from xL have xL2: "x' \<notin> set L" by auto
     from xL have xx: "x' \<noteq> x" by simp
-    from xL have xgp: "lookup x' \<Gamma>' = None" using not_dom_lookup_none by auto
-    from xgp have "\<Gamma>' \<preceq> ((x',T1)#\<Gamma>')" by simp
-    with wtv env_weakening[of \<Gamma>' v B "(x',T1)#\<Gamma>'"] 
-    have wtv2: "(x',T1)#\<Gamma>' \<turnstile> v : B" by blast 
+    from xL have xgp: "lookup x' Γ' = None" using not_dom_lookup_none by auto
+    from xgp have "Γ' \<preceq> ((x',T1)::Γ')" by simp
+    with wtv env_weakening[of Γ' v B "(x',T1)::Γ'"] 
+    have wtv2: "(x',T1)::Γ' ⊢ v : B" by blast 
     from wt_lambda lx2 rb2 xL2 wtv2 xx
-    have 1: "(x',T1)#\<Gamma>' \<turnstile> [x\<mapsto>v]({0\<rightarrow>FVar x'} e) : T2" by auto
+    have 1: "(x',T1)::Γ' ⊢ [[x~>v]](∆x'·e) : T2" by auto
     from wtv xx  subst_permute
-    have "[x\<mapsto>v]({0\<rightarrow>FVar x'}e) = {0\<rightarrow>FVar x'}([x\<mapsto>v]e)" by auto
-    with 1 show "(x',T1)#\<Gamma>' \<turnstile> ({0\<rightarrow>FVar x'}([x\<mapsto>v]e)) : T2" by simp
+    have "[[x~>v]](∆x'·e) = ∆x'·([[x~>v]]e)" by auto
+    with 1 show "(x',T1)::Γ' ⊢ (∆x'·([[x~>v]]e)) : T2" by simp
   qed
-  thus "\<Gamma>' \<turnstile> [x\<mapsto>v]LambdaE e : T1 \<rightarrow> T2" by simp
+  thus "Γ' ⊢ [[x~>v]]LambdaE e : T1 \<rightarrow> T2" by simp
 next
-  case (wt_app \<Gamma> e1 T T' e2 x B \<Gamma>' v)
-  thus "\<Gamma>' \<turnstile> [x\<mapsto>v]AppE e1 e2 : T'" by auto 
+  case (wt_app Γ e1 T T' e2 x B Γ' v)
+  thus "Γ' ⊢ [[x~>v]]AppE e1 e2 : T'" by auto 
 qed
 
 lemma substitution_preserves_types:
   fixes M::exp and v::exp
-  assumes wtm: "(x,B)#\<Gamma> \<turnstile> M : A" and vb: "\<Gamma> \<turnstile> v : B"
-  shows "\<Gamma> \<turnstile> [x \<mapsto> v]M : A" 
-  using wtm vb subst_pres_types[of "(x,B)#\<Gamma>" M A x B \<Gamma> v] by auto
+  assumes wtm: "(x,B)::Γ ⊢ M : A" and vb: "Γ ⊢ v : B"
+  shows "Γ ⊢ [[x~>v]]M : A" 
+  using wtm vb subst_pres_types[of "(x,B)::Γ" M A x B Γ v] by auto
 
 lemma msubst_preserves_types:
-  fixes M::exp and \<rho>::env assumes wtm: "\<Gamma>1@\<Gamma>2 \<turnstile> M : A" and sr: "\<Gamma>1 \<turnstile> \<rho>"
-  shows "\<Gamma>2 \<turnstile> [\<rho>]M : A" using wtm sr
-proof (induction \<rho> arbitrary: \<Gamma>1 \<Gamma>2 M A)
-  case (Nil \<Gamma>1 \<Gamma>2 M A) thus "\<Gamma>2 \<turnstile> [[]] M : A" by auto
+  fixes M::exp and ρ::env assumes wtm: "Γ1++Γ2 ⊢ M : A" and sr: "Γ1 ⊢ ρ"
+  shows "Γ2 ⊢ [ρ]M : A" using wtm sr
+proof (induction ρ arbitrary: Γ1 Γ2 M A)
+  case (Nil Γ1 Γ2 M A) thus "Γ2 ⊢ [[]] M : A" by auto
 next
-  case (Cons a \<rho> \<Gamma>1 \<Gamma>2 M A)
-  show "\<Gamma>2 \<turnstile> [(a#\<rho>)] M : A"
+  case (Cons a ρ Γ1 Γ2 M A)
+  show "Γ2 ⊢ [(a::ρ)] M : A"
   proof (cases a)
     fix x v assume a: "a = (x,v)"
-    from a have 1: "[(a#\<rho>)]M = [\<rho>] ([x\<mapsto>v] M)" by simp
-    from Cons a obtain \<Gamma>1'::ty_env and B::ty where g1: "\<Gamma>1 = (x,B)#\<Gamma>1'" 
-      and wtv: "[] \<turnstile> v : B" and g1pr: "\<Gamma>1' \<turnstile> \<rho>" by auto
-    from Cons g1 have wtm: "(x,B)#(\<Gamma>1'@\<Gamma>2) \<turnstile> M : A" by simp
-    from wtv env_weakening[of "[]"]  have wtv2: "\<Gamma>1'@\<Gamma>2 \<turnstile> v : B" by auto
-    from wtm wtv2 have wtm2: "\<Gamma>1'@\<Gamma>2 \<turnstile> [x\<mapsto>v]M : A"
+    from a have 1: "[(a::ρ)]M = [ρ] ([[x~>v]] M)" by simp
+    from Cons a obtain Γ1'::ty_env and B::ty where g1: "Γ1 = (x,B)::Γ1'" 
+      and wtv: "[] ⊢ v : B" and g1pr: "Γ1' ⊢ ρ" by auto
+    from Cons g1 have wtm: "(x,B)::(Γ1'++Γ2) ⊢ M : A" by simp
+    from wtv env_weakening[of "[]"]  have wtv2: "Γ1'++Γ2 ⊢ v : B" by auto
+    from wtm wtv2 have wtm2: "Γ1'++Γ2 ⊢ [[x~>v]]M : A"
       using substitution_preserves_types by blast
-    from wtm2 Cons g1pr have "\<Gamma>2 \<turnstile> [\<rho>]([x\<mapsto>v]M) : A" by blast
+    from wtm2 Cons g1pr have "Γ2 ⊢ [ρ]([[x~>v]]M) : A" by blast
     with a show ?thesis by simp
   qed
 qed
@@ -904,41 +997,41 @@ qed
 
 section "Adequacy of Locally Nameless Type System"
 
-lemma adequacy1: fixes e::exp assumes wte: "\<Gamma> \<turnstile> e : T" shows "\<Gamma> \<turnstile>o e : T"
-using wte apply (induction \<Gamma> e T) apply force apply force apply force
+lemma adequacy1: fixes e::exp assumes wte: "Γ ⊢ e : T" shows "Γ ⊢o e : T"
+using wte apply (induction Γ e T) apply force apply force apply force
 apply force defer apply force
 proof -
-  case (wt_lambda L T1 \<Gamma> e T2)
+  case (wt_lambda L T1 Γ e T2)
   let ?X = "Suc (max (list_max L) (list_max (FV e)))"
-  show "\<Gamma> \<turnstile>o LambdaE e : T1 \<rightarrow> T2"
+  show "Γ ⊢o LambdaE e : T1 \<rightarrow> T2"
   proof
     show "?X \<notin> set (FV e)" using list_max_fresh[of "FV e" "?X"] by auto
   next
     have "?X \<notin> set L" using list_max_fresh by auto
-    with wt_lambda show "(?X,T1)#\<Gamma> \<turnstile>o ({0\<rightarrow>FVar ?X} e) : T2" by blast
+    with wt_lambda show "(?X,T1)::Γ ⊢o (∆?X·e) : T2" by blast
   qed
 qed
 
-lemma adequacy2: fixes e::exp assumes wte: "\<Gamma> \<turnstile>o e : T" shows "\<Gamma> \<turnstile> e : T"
-using wte apply (induction \<Gamma> e T rule: wt.induct) apply force 
+lemma adequacy2: fixes e::exp assumes wte: "Γ ⊢o e : T" shows "Γ ⊢ e : T"
+using wte apply (induction Γ e T rule: wt.induct) apply force 
 apply force apply force apply force defer apply force
 proof -
-  case (wt_l x e T1 \<Gamma> T2)
+  case (wt_l x e T1 Γ T2)
   from wt_l have xfv: "x \<notin> set (FV e)" and
-    1: "(x,T1)#\<Gamma> \<turnstile> ({0\<rightarrow>FVar x}e) : T2" by auto
-  show "\<Gamma> \<turnstile> LambdaE e : T1 \<rightarrow> T2"
+    1: "(x,T1)::Γ ⊢ (∆x·e) : T2" by auto
+  show "Γ ⊢ LambdaE e : T1 \<rightarrow> T2"
   proof clarify
-    fix x' assume xL: "x' \<notin> set (FV e @ map fst \<Gamma>)"
-    from xL not_dom_lookup_none[of x' \<Gamma>] 
-    have lxg: "lookup x' \<Gamma> = None" by simp
-    hence rb: "remove_bind x ((x,T1)#\<Gamma>) ((x',T1)#\<Gamma>)" by auto 
-    have lxg2: "lookup x ((x,T1)#\<Gamma>) = Some T1" by simp
-    have wtxp: "(x',T1)#\<Gamma> \<turnstile> FVar x' : T1" by auto
+    fix x' assume xL: "x' \<notin> set (FV e ++ map fst Γ)"
+    from xL not_dom_lookup_none[of x' Γ] 
+    have lxg: "lookup x' Γ = None" by simp
+    hence rb: "remove_bind x ((x,T1)::Γ) ((x',T1)::Γ)" by auto 
+    have lxg2: "lookup x ((x,T1)::Γ) = Some T1" by simp
+    have wtxp: "(x',T1)::Γ ⊢ FVar x' : T1" by auto
     from 1 lxg2 rb wtxp subst_pres_types
-    have 2: "(x',T1)#\<Gamma> \<turnstile> [x\<mapsto>FVar x']({0\<rightarrow>FVar x}e) : T2" by blast
-    from xfv have 3: "{0\<rightarrow>FVar x'}e = [x\<mapsto>FVar x']({0\<rightarrow>FVar x}e)"
+    have 2: "(x',T1)::Γ ⊢ [[x~>FVar x']](∆x·e) : T2" by blast
+    from xfv have 3: "∆x'·e = [[x~>FVar x']](∆x·e)"
       using decompose_subst[of x e] by blast
-    from 2 3 show "(x',T1)#\<Gamma> \<turnstile> ({0\<rightarrow>FVar x'}e) : T2" by simp
+    from 2 3 show "(x',T1)::Γ ⊢ (∆x'·e) : T2" by simp
   qed
 qed
 
@@ -948,13 +1041,13 @@ section "Termination via a Logical Relations Proof"
 subsection "The Logical Predicates"
 
 
-fun WTE :: "ty \<Rightarrow> exp set" and WTV :: "ty \<Rightarrow> exp set" where
+fun WTE :: "ty => exp set" and WTV :: "ty => exp set" where
   "WTE T = { e. \<exists> n v. interp e n = Res v \<and> v \<in> WTV T }" |
 
   "WTV IntT = { v. \<exists> i. v = Const (IntC i) }" |
   "WTV BoolT = {v. \<exists> b. v = Const (BoolC b) }" |
-  "WTV (T1\<rightarrow>T2) = {f. \<exists> e. f = LambdaE e \<and> [] \<turnstile>o f : T1 \<rightarrow> T2
-     \<and> (\<forall>v\<in>WTV T1.\<exists> n v'. interp ({0\<rightarrow>v} e) n = Res v' \<and> v'\<in>WTV T2)}"
+  "WTV (T1\<rightarrow>T2) = {f. \<exists> e. f = LambdaE e \<and> [] ⊢o f : T1 \<rightarrow> T2
+     \<and> (\<forall>v\<in>WTV T1.\<exists> n v'. interp (∆∆v·e) n = Res v' \<and> v'\<in>WTV T2)}"
 
 
 lemma WTE_intro[intro]: 
@@ -962,10 +1055,10 @@ lemma WTE_intro[intro]:
   shows "e \<in> WTE T" using ie vt by auto
 
 
-fun WTENV :: "ty_env \<Rightarrow> env set" where
+fun WTENV :: "ty_env => env set" where
   "WTENV [] = { [] }" |
-  "WTENV ((x,T)#\<Gamma>) = {\<rho>. \<exists> v \<rho>'. \<rho>=(x,v)#\<rho>' 
-                          \<and> v \<in> WTV T \<and> \<rho>' \<in> WTENV \<Gamma> }"
+  "WTENV ((x,T)::Γ) = {ρ. \<exists> v ρ'. ρ=(x,v)::ρ' 
+                          \<and> v \<in> WTV T \<and> ρ' \<in> WTENV Γ }"
 
 subsection "Properties of WTV and WTE"
 
@@ -973,13 +1066,13 @@ lemma WTV_implies_WTE:
   assumes wtv: "v \<in> WTV T" shows "v \<in> WTE T"
   using wtv apply (cases T) apply auto by (rule_tac x="Suc 0" in exI, force)+
 
-lemma WTV_implies_WT: assumes wtv: "v \<in> WTV T" shows "[] \<turnstile>o v : T"
+lemma WTV_implies_WT: assumes wtv: "v \<in> WTV T" shows "[] ⊢o v : T"
   using wtv by (cases T) auto
 
 lemma wtenv_lookup: 
-  assumes lg: "lookup x \<Gamma> = Some T" and wtenv: "\<rho> \<in> WTENV \<Gamma>" 
-  shows "\<exists> v. lookup x \<rho> = Some v \<and> v \<in> WTV T"
-  using lg wtenv by (induction \<Gamma> arbitrary: x \<rho>) auto
+  assumes lg: "lookup x Γ = Some T" and wtenv: "ρ \<in> WTENV Γ" 
+  shows "\<exists> v. lookup x ρ = Some v \<and> v \<in> WTV T"
+  using lg wtenv by (induction Γ arbitrary: x ρ) auto
 
 
 subsection "The Main Lemma and Theorem"
@@ -991,56 +1084,56 @@ lemma prim_type_safe:
 
 
 lemma wt_dom_fv2: fixes v::exp and T::ty 
-  assumes wt: "[] \<turnstile> v : T" shows "FV v = []"
+  assumes wt: "[] ⊢ v : T" shows "FV v = []"
   using wt wt_dom_fv[of "[]" v T] adequacy1[of "[]" v T] by auto
 
 
 lemma WT_implies_WTE: fixes e::exp
-  assumes wt: "\<Gamma> \<turnstile> e : T" and wtenv: "\<rho> \<in> WTENV \<Gamma>" and wt_env: "\<Gamma> \<turnstile> \<rho>"
-  shows "[\<rho>]e \<in> WTE T"
+  assumes wt: "Γ ⊢ e : T" and wtenv: "ρ \<in> WTENV Γ" and wt_env: "Γ ⊢ ρ"
+  shows "[ρ]e \<in> WTE T"
 using wt wtenv wt_env
-proof (induction \<Gamma> e T arbitrary: \<rho>)
-  case (wt_const c T \<Gamma> \<rho>)
-  from this show "[\<rho>]Const c \<in> WTE T" 
+proof (induction Γ e T arbitrary: ρ)
+  case (wt_const c T Γ ρ)
+  from this show "[ρ]Const c \<in> WTE T" 
     apply (case_tac c, auto) apply (rule_tac x="Suc 0" in exI, force)+ done
 next
-  case (wt_prim \<Gamma> e T1 p T2 \<rho>)
-  from wt_prim have "[\<rho>]e \<in> WTE T1" by auto
+  case (wt_prim Γ e T1 p T2 ρ)
+  from wt_prim have "[ρ]e \<in> WTE T1" by auto
   from this obtain v n where 
-    ie: "interp ([\<rho>]e) n = Res v" and wtv: "v \<in> WTV T1" by auto
+    ie: "interp ([ρ]e) n = Res v" and wtv: "v \<in> WTV T1" by auto
   from wt_prim have pt: "prim_type p = (T1,T2)" by blast
   from pt wtv obtain c where v: "v = Const c" and ct: "const_type c = T1"
     by (case_tac p) auto
   from pt v ct obtain c' where ip: "eval_prim p c = Result c'"
     and ctp: "const_type c' = T2" using prim_type_safe by blast
-  from ie ip ctp v show "[\<rho>]Prim p e \<in> WTE T2"
+  from ie ip ctp v show "[ρ]Prim p e \<in> WTE T2"
     apply (case_tac c', auto) apply (rule_tac x="Suc n" in exI, force)+ done
 next
-  case (wt_if \<Gamma> e1 e2 T e3 \<rho>)
-  from wt_if have "[\<rho>]e1 \<in> WTE BoolT" by auto
+  case (wt_if Γ e1 e2 T e3 ρ)
+  from wt_if have "[ρ]e1 \<in> WTE BoolT" by auto
   from this obtain v1 n1 where 
-    ie1: "interp ([\<rho>]e1) n1 = Res v1" and wtv1: "v1 \<in> WTV BoolT" by auto
+    ie1: "interp ([ρ]e1) n1 = Res v1" and wtv1: "v1 \<in> WTV BoolT" by auto
   from wtv1 obtain b where v1: "v1 = Const (BoolC b)" by auto
-  show "[\<rho>]IfE e1 e2 e3 \<in> WTE T"
+  show "[ρ]IfE e1 e2 e3 \<in> WTE T"
   proof (cases b)
     case True
-    from wt_if have "[\<rho>]e2 \<in> WTE T" by auto
+    from wt_if have "[ρ]e2 \<in> WTE T" by auto
     from this obtain v2 n2 where 
-      ie2: "interp ([\<rho>]e2) n2 = Res v2" and wtv2: "v2 \<in> WTV T" by auto
+      ie2: "interp ([ρ]e2) n2 = Res v2" and wtv2: "v2 \<in> WTV T" by auto
     show ?thesis
-    proof (cases "n1 \<le> n2")
-      assume "n1 \<le> n2"
-      with ie1 interp_mono have "interp ([\<rho>]e1) n2 = Res v1" by blast
-      with ie2 True v1 have "interp ([\<rho>]IfE e1 e2 e3) (Suc n2) = Res v2" by simp
+    proof (cases "n1 <= n2")
+      assume "n1 <= n2"
+      with ie1 interp_mono have "interp ([ρ]e1) n2 = Res v1" by blast
+      with ie2 True v1 have "interp ([ρ]IfE e1 e2 e3) (Suc n2) = Res v2" by simp
       with wtv2 show ?thesis by blast
     next
-      assume "\<not> n1 \<le> n2" -- "This case is the mirror image of the above case"
+      assume "~(n1 <= n2)" -- "This case is the mirror image of the above case"
 
 (*<*)
-      from this have n12: "n2 \<le> n1" by simp
-      from ie2 n12 interp_mono have ie2b: "interp ([\<rho>]e2) n1 = Res v2"  by blast
+      from this have n12: "n2 <= n1" by simp
+      from ie2 n12 interp_mono have ie2b: "interp ([ρ]e2) n1 = Res v2"  by blast
       from ie1 ie2b True v1
-      have iif: "interp ([\<rho>]IfE e1 e2 e3) (Suc n1) = Res v2" by simp
+      have iif: "interp ([ρ]IfE e1 e2 e3) (Suc n1) = Res v2" by simp
       from iif wtv2 show ?thesis by blast
 (*>*)
     qed
@@ -1048,122 +1141,122 @@ next
     case False -- "This case is the mirror image of the case for True"
 
 (*<*)
-    from wt_if have "[\<rho>]e3 \<in> WTE T" by auto
+    from wt_if have "[ρ]e3 \<in> WTE T" by auto
     from this obtain v2 n2 where 
-      ie2: "interp ([\<rho>]e3) n2 = Res v2" and wtv2: "v2 \<in> WTV T" by auto
+      ie2: "interp ([ρ]e3) n2 = Res v2" and wtv2: "v2 \<in> WTV T" by auto
     show ?thesis
-    proof (cases "n1 \<le> n2")
-      assume n12: "n1 \<le> n2"
-      from ie1 n12 interp_mono have ie1b: "interp ([\<rho>]e1) n2 = Res v1"  by blast
+    proof (cases "n1 <= n2")
+      assume n12: "n1 <= n2"
+      from ie1 n12 interp_mono have ie1b: "interp ([ρ]e1) n2 = Res v1"  by blast
       from ie1b ie2 False v1
-      have iif: "interp ([\<rho>]IfE e1 e2 e3) (Suc n2) = Res v2" by simp
+      have iif: "interp ([ρ]IfE e1 e2 e3) (Suc n2) = Res v2" by simp
       from iif wtv2 show ?thesis by blast
     next
-      assume "\<not> n1 \<le> n2"
-      from this have n12: "n2 \<le> n1" by simp
-      from ie2 n12 interp_mono have ie2b: "interp ([\<rho>]e3) n1 = Res v2" by blast
+      assume "~(n1 <= n2)"
+      from this have n12: "n2 <= n1" by simp
+      from ie2 n12 interp_mono have ie2b: "interp ([ρ]e3) n1 = Res v2" by blast
       from ie1 ie2b False v1
-      have iif: "interp ([\<rho>]IfE e1 e2 e3) (Suc n1) = Res v2" by simp
+      have iif: "interp ([ρ]IfE e1 e2 e3) (Suc n1) = Res v2" by simp
       from iif wtv2 show ?thesis by blast
     qed
 (*>*)
   qed
 next
-  case (wt_var x \<Gamma> T \<rho>)
-  from this wtenv_lookup obtain v where lx: "lookup x \<rho> = Some v" 
+  case (wt_var x Γ T ρ)
+  from this wtenv_lookup obtain v where lx: "lookup x ρ = Some v" 
     and vt: "v \<in> WTV T" by blast
-  from wt_var lx wt_env_lookup[of x \<Gamma> T \<rho>]  have wtv: "[] \<turnstile> v : T" by auto
-  from lx wtv have "[\<rho>]FVar x = v" using msubst_var1 wt_dom_fv2 by simp
-  with vt have "[\<rho>] FVar x \<in> WTV T" by simp
-  with WTV_implies_WTE show "[\<rho>] FVar x \<in> WTE T" by auto
+  from wt_var lx wt_env_lookup[of x Γ T ρ]  have wtv: "[] ⊢ v : T" by auto
+  from lx wtv have "[ρ]FVar x = v" using msubst_var1 wt_dom_fv2 by simp
+  with vt have "[ρ] FVar x \<in> WTV T" by simp
+  with WTV_implies_WTE show "[ρ] FVar x \<in> WTE T" by auto
 next
-  case (wt_lambda L T1 \<Gamma> e T2 \<rho>)
-  from wt_lambda have gr: "\<Gamma> \<turnstile> \<rho>" by simp
-  from wt_lambda have wtr: "\<rho> \<in> WTENV \<Gamma>" by simp
-  let ?L = "L @ (FV e) @ (FV ([\<rho>]e)) @ (map fst \<Gamma>) @ (map fst \<rho>)"
-  have "[] \<turnstile> LambdaE ([\<rho>]e) : T1 \<rightarrow> T2" 
+  case (wt_lambda L T1 Γ e T2 ρ)
+  from wt_lambda have gr: "Γ ⊢ ρ" by simp
+  from wt_lambda have wtr: "ρ \<in> WTENV Γ" by simp
+  let ?L = "L ++ (FV e) ++ (FV ([ρ]e)) ++ (map fst Γ) ++ (map fst ρ)"
+  have "[] ⊢ LambdaE ([ρ]e) : T1 \<rightarrow> T2" 
   proof
-    show "\<forall>x. x \<notin> set ?L \<longrightarrow> [(x, T1)] \<turnstile> ({0\<rightarrow>FVar x} [\<rho>]e) : T2" 
+    show "\<forall>x. x \<notin> set ?L \<longrightarrow> [(x, T1)] ⊢ (∆x·[ρ]e) : T2" 
     proof clarify
       fix x assume xl2: "x \<notin> set ?L"
-      let ?G1 = "[(x,T1)]@\<Gamma>" and ?G2 = "\<Gamma>@[(x,T1)]"
-      from xl2 wt_lambda have 3: "?G1 \<turnstile> ({0\<rightarrow>FVar x}e) : T2" by auto
+      let ?G1 = "[(x,T1)]++Γ" and ?G2 = "Γ++[(x,T1)]"
+      from xl2 wt_lambda have 3: "?G1 ⊢ (∆x·e) : T2" by auto
       from xl2 have 4: "?G1 \<preceq> ?G2" using weaken_cons_snoc by auto
-      from 3 4 have "?G2 \<turnstile> ({0\<rightarrow>FVar x}e) : T2" using env_weakening by blast
-      with gr have 5: "[(x,T1)] \<turnstile> [\<rho>]({0\<rightarrow>FVar x}e) : T2" 
+      from 3 4 have "?G2 ⊢ (∆x·e) : T2" using env_weakening by blast
+      with gr have 5: "[(x,T1)] ⊢ [ρ](∆x·e) : T2" 
         using msubst_preserves_types by blast
-      from xl2 have "assoc_dom \<rho> \<inter> set (FV (FVar x)) = {}" by simp
+      from xl2 have "assoc_dom ρ \<inter> set (FV (FVar x)) = {}" by simp
       with 5 gr msubst_permute 
-      show "[(x,T1)] \<turnstile> ({0\<rightarrow>FVar x}([\<rho>]e)) : T2" by simp
+      show "[(x,T1)] ⊢ (∆x·([ρ]e)) : T2" by simp
     qed  
   qed
-  hence wtlam: "[] \<turnstile>o LambdaE ([\<rho>]e) : T1 \<rightarrow> T2" by (rule adequacy1)
-  have ibody: "\<forall>v\<in>WTV T1.\<exists>n v'. interp({0\<rightarrow>v}[\<rho>]e) n=Res v' \<and> v'\<in>WTV T2"
+  hence wtlam: "[] ⊢o LambdaE ([ρ]e) : T1 \<rightarrow> T2" by (rule adequacy1)
+  have ibody: "\<forall>v\<in>WTV T1.\<exists>n v'. interp(∆∆v·[ρ]e) n=Res v' \<and> v'\<in>WTV T2"
   proof
     fix v assume vt1: "v \<in> WTV T1"
-    let ?X = "Suc (list_max [list_max L, list_max (FV e), list_max (FV ([\<rho>]e)), 
-                           list_max (map fst \<Gamma>), list_max (map fst \<rho>)])"
+    let ?X = "Suc (list_max [list_max L, list_max (FV e), list_max (FV ([ρ]e)), 
+                           list_max (map fst Γ), list_max (map fst ρ)])"
     have xfv: "?X \<notin> set (FV e)" and xl: "?X \<notin> set L" 
       using list_max_fresh by auto
-    from vt1 wtr have wtr2: "(?X,v)#\<rho> \<in> WTENV ((?X,T1)#\<Gamma>)" by simp
-    from vt1 WTV_implies_WT adequacy2 have "[] \<turnstile> v : T1" by blast
-    with gr have gr2: "((?X,T1)#\<Gamma>) \<turnstile> (?X,v)#\<rho>" by blast
-    let ?E = "[((?X,v)#\<rho>)]({0\<rightarrow>FVar ?X}e)"
+    from vt1 wtr have wtr2: "(?X,v)::ρ \<in> WTENV ((?X,T1)::Γ)" by simp
+    from vt1 WTV_implies_WT adequacy2 have "[] ⊢ v : T1" by blast
+    with gr have gr2: "((?X,T1)::Γ) ⊢ (?X,v)::ρ" by blast
+    let ?E = "[((?X,v)::ρ)](∆?X·e)"
     from wt_lambda xl wtr2 gr2 have IH: "?E \<in> WTE T2" by blast
     from IH obtain v' n where ie: "interp ?E n = Res v'" and 
       wtvp: "v' \<in> WTV T2" by auto
     from vt1 have "FV v = []" 
       using WTV_implies_WT[of v T1] wt_dom_fv[of "[]" v T1] by simp
-    hence drfv: "assoc_dom \<rho> \<inter> set (FV v) = {}" by simp
-    have "?E = [\<rho>]([?X\<mapsto>v]({0\<rightarrow>FVar ?X}e))" by simp
-    also with xfv have "... = [\<rho>]({0\<rightarrow>v}e)" 
+    hence drfv: "assoc_dom ρ \<inter> set (FV v) = {}" by simp
+    have "?E = [ρ]([[?X~>v]](∆?X·e))" by simp
+    also with xfv have "... = [ρ](∆∆v·e)" 
       using decompose_subst[of "?X" e 0 v] by simp
-    finally have "?E = {0\<rightarrow>v}[\<rho>]e"  
-      using drfv gr msubst_permute[of \<rho> v \<Gamma> 0 e] by simp
+    finally have "?E = ∆∆v·[ρ]e"  
+      using drfv gr msubst_permute[of ρ v Γ 0 e] by simp
     with ie wtvp
-    show "\<exists> n v'. interp({0\<rightarrow>v}[\<rho>]e) n = Res v' \<and> v' \<in> WTV T2" by auto
+    show "\<exists> n v'. interp(∆∆v·[ρ]e) n = Res v' \<and> v' \<in> WTV T2" by auto
   qed
-  from wtlam ibody have lv: "LambdaE ([\<rho>]e) \<in> WTV (T1 \<rightarrow> T2)" by simp
-  have il: "interp (LambdaE ([\<rho>]e)) (Suc 0) = Res (LambdaE ([\<rho>]e))" by simp
-  from il lv have "LambdaE ([\<rho>]e) \<in> WTE (T1 \<rightarrow> T2)" by blast
-  thus "[\<rho>](LambdaE e) \<in> WTE (T1 \<rightarrow> T2)" by simp
+  from wtlam ibody have lv: "LambdaE ([ρ]e) \<in> WTV (T1 \<rightarrow> T2)" by simp
+  have il: "interp (LambdaE ([ρ]e)) (Suc 0) = Res (LambdaE ([ρ]e))" by simp
+  from il lv have "LambdaE ([ρ]e) \<in> WTE (T1 \<rightarrow> T2)" by blast
+  thus "[ρ](LambdaE e) \<in> WTE (T1 \<rightarrow> T2)" by simp
 next
-  case (wt_app \<Gamma> e1 T T' e2 \<rho>)
-  from wt_app have "\<Gamma> \<turnstile> e1 : T \<rightarrow> T'" by simp
-  from wt_app have IH1: "[\<rho>]e1 \<in> WTE (T \<rightarrow> T')" by simp
-  from wt_app have IH2: "[\<rho>]e2 \<in> WTE T" by simp
-  from IH1 obtain v1 n1 where ie1: "interp ([\<rho>]e1) n1 = Res v1" 
+  case (wt_app Γ e1 T T' e2 ρ)
+  from wt_app have "Γ ⊢ e1 : T \<rightarrow> T'" by simp
+  from wt_app have IH1: "[ρ]e1 \<in> WTE (T \<rightarrow> T')" by simp
+  from wt_app have IH2: "[ρ]e2 \<in> WTE T" by simp
+  from IH1 obtain v1 n1 where ie1: "interp ([ρ]e1) n1 = Res v1" 
     and v1t: "v1 \<in> WTV (T\<rightarrow>T')" by force 
-  from IH2 obtain v2 n2 where ie2: "interp ([\<rho>]e2) n2 = Res v2" 
+  from IH2 obtain v2 n2 where ie2: "interp ([ρ]e2) n2 = Res v2" 
     and v2t: "v2 \<in> WTV T" by (cases T) auto
   from v1t obtain e where v1: "v1 = LambdaE e" and
-    app: "\<forall>v\<in>WTV T.\<exists>n v'. interp ({0\<rightarrow>v}e) n =Res v' \<and> v'\<in>WTV T'" by auto
-  from v2t app obtain n3 v' where ie3: "interp ({0\<rightarrow>v2}e) n3 = Res v'"
+    app: "\<forall>v\<in>WTV T.\<exists>n v'. interp (∆∆v·e) n =Res v' \<and> v'\<in>WTV T'" by auto
+  from v2t app obtain n3 v' where ie3: "interp (∆∆v2·e) n3 = Res v'"
     and vpt: "v' \<in> WTV T'" by auto
   let ?N = "n1 + n2 + n3"
-  have n1n: "n1 \<le> ?N" and n2n: "n2 \<le> ?N" and n3n: "n3 \<le> ?N" by auto
-  from ie1 n1n ie2 n2n ie3 n3n have ie1b: "interp ([\<rho>]e1) ?N = Res v1" and
-    ie2b: "interp ([\<rho>]e2) ?N = Res v2" and 
-    ie3b: "interp ({0\<rightarrow>v2}e) ?N = Res v'" using interp_mono by blast+
+  have n1n: "n1 <= ?N" and n2n: "n2 <= ?N" and n3n: "n3 <= ?N" by auto
+  from ie1 n1n ie2 n2n ie3 n3n have ie1b: "interp ([ρ]e1) ?N = Res v1" and
+    ie2b: "interp ([ρ]e2) ?N = Res v2" and 
+    ie3b: "interp (∆∆v2·e) ?N = Res v'" using interp_mono by blast+
   from ie1b ie2b ie3b v1
-  have "interp (AppE ([\<rho>]e1) ([\<rho>]e2)) (Suc ?N) = Res v'" by auto
-  with vpt have "AppE ([\<rho>]e1) ([\<rho>]e2) \<in> WTE T'" by blast
-  thus "[\<rho>]AppE e1 e2 \<in> WTE T'" by simp
+  have "interp (AppE ([ρ]e1) ([ρ]e2)) (Suc ?N) = Res v'" by auto
+  with vpt have "AppE ([ρ]e1) ([ρ]e2) \<in> WTE T'" by blast
+  thus "[ρ]AppE e1 e2 \<in> WTE T'" by simp
 qed
 
 theorem WT_implies_iterp:
-  fixes e::exp assumes wt: "[] \<turnstile> e : T"
-  shows "\<exists> v n. interp e n = Res v \<and> [] \<turnstile> v : T"
+  fixes e::exp assumes wt: "[] ⊢ e : T"
+  shows "\<exists> v n. interp e n = Res v \<and> [] ⊢ v : T"
 proof -
   let ?R = "[]" and ?G = "[]"
   have 1: "?R \<in> WTENV []" by auto
-  have 2: "[] \<turnstile> []" by auto
+  have 2: "[] ⊢ []" by auto
   from wt 1 2 have "[?R]e \<in> WTE T" by (rule WT_implies_WTE)
   hence 3: "e \<in> WTE T" by simp
   from 3 obtain v n where ev: "interp e n = Res v" and
     vt: "v \<in> WTV T" by auto
-  from vt have "[] \<turnstile>o v : T" by (rule WTV_implies_WT)
-  hence "[] \<turnstile> v : T" by (rule adequacy2)
+  from vt have "[] ⊢o v : T" by (rule WTV_implies_WT)
+  hence "[] ⊢ v : T" by (rule adequacy2)
   with ev show ?thesis by blast
 qed
 *)
