LNVarMap.v
@@ -1,0 +1,103 @@
+(* ~~~~~~~~~~~~~~~~~~~~~~~~~~~~~~~~~~~~~~~~~~~~~~~~~~~~~~~~~~ *)
+(** * Finite maps from variables/names, for use with the locally nameless style. *)
+(* ~~~~~~~~~~~~~~~~~~~~~~~~~~~~~~~~~~~~~~~~~~~~~~~~~~~~~~~~~~ *)
+(* [Coq.Classes.EquivDec] is Coq 8.3 only *)
+Require Import Coq.Lists.ListSet.
+Require Import Coq.Lists.List.
+Require Import Coq.Classes.EquivDec.
+
+Require Import WrengrUtil.CoqExtras.ListSet.
+Require Export LNSet.
+Require Export LNVar.
+
+(* ~~~~~~~~~~~~~~~~~~~~~~~~~~~~~~~~~~~~~~~~~~~~~~~~~~~~~~~~~~ *)
+Section LNVarMap.
+Context  {Var : Set}.
+Context `{VT : VarType Var}.
+Implicit Type x y z : Var.
+
+Context  {A : Type}.
+Implicit Type a b c : A.
+
+
+(* TODO: abstract over the fact that we're implementing [VarMap] with [list]. *)
+Definition VarMap := list (Var * A).
+Implicit Type ρ Γ : VarMap.
+
+
+Fixpoint assoc_dom Γ : set Var :=
+    match Γ with
+    | nil       => \{}
+    | (x,_)::Γ' => x \a assoc_dom Γ'
+    end.
+
+
+Fixpoint lookup x Γ : option A :=
+    match Γ with
+    | nil          => None
+    | (y,a)::Γ' =>
+        if equiv_dec x y
+        then Some a
+        else lookup x Γ'
+    end.
+
+
+(* ~~~~~~~~~~~~~~~~~~~~~~~~~~~~~~~~~~~~~~~~~~~~~~~~~~~~~~~~~~ *)
+Lemma lookup_app
+    : forall {Γ} Γ' {x a}
+    ,  lookup x Γ = Some a
+    -> lookup x (Γ++Γ') = Some a.
+Proof.
+  intros Γ; induction Γ as [| (y,b) Γ IHΓ]; simpl; intros Γ' x a H;
+    [ discriminate H
+    | destruct (equiv_dec x y); [| apply IHΓ ]; assumption
+    ].
+Qed.
+
+
+(* BUG: why can't we use the [[(x,a)]] notation here?! *)
+Lemma lookup_app_none
+    : forall {Γ x} a
+    ,  lookup x Γ = None
+    -> lookup x (Γ ++ ((x,a)::nil)) = Some a.
+Proof.
+  intros Γ; induction Γ as [| (y,b) Γ IHΓ]; simpl; intros x a H;
+    [ destruct (equiv_dec x x); congruence
+    | destruct (equiv_dec x y); [ discriminate | apply IHΓ; assumption ]
+    ].
+Qed.
+
+
+Lemma not_dom_lookup_none
+    : forall {Γ x}
+    ,  x \notin assoc_dom Γ
+    -> lookup x Γ = None.
+Proof.
+  intros Γ; induction Γ as [| (y,b) Γ IHΓ]; simpl; intros x H;
+    [ reflexivity
+    | destruct (equiv_dec x y);
+      [ contradiction H | apply IHΓ ];
+      auto with listset
+    ].
+Qed.
+
+
+Lemma lookup_dom
+    : forall {Γ x a}
+    ,  lookup x Γ = Some a
+    -> x \in assoc_dom Γ.
+Proof.
+  intros Γ; induction Γ as [| (y,b) Γ IHΓ]; simpl; intros x a H;
+    [ discriminate
+    | destruct (equiv_dec x y); [| pose (IHΓ _ _ H) ]; auto with listset
+    ].
+Qed.
+
+
+End LNVarMap.
+
+(* Undo the implicitness of [Var] and [A] for [VarMap]. *)
+Implicit Arguments VarMap [].
+
+(* ~~~~~~~~~~~~~~~~~~~~~~~~~~~~~~~~~~~~~~~~~~~~~~~~~~~~~~~~~~ *)
+(* ~~~~~~~~~~~~~~~~~~~~~~~~~~~~~~~~~~~~~~~~~~~~~~~~~~~~~ fin. *)
